theories/church_types.v
@@ -1,0 +1,58 @@
+Require Export stlc_types.
+
+
+(** * Church Implementation *)
+
+Module TyChurch <: TY.
+  Inductive tyc : Set :=
+    | tyc_prp : tyc
+    | tyc_arr : tyc -> tyc -> tyc
+    | tyc_obj : tyc.
+
+  Definition ty := tyc.
+  Definition ty_prp := tyc_prp.
+  Definition ty_arr := tyc_arr.
+
+  Definition ty_other t : Prop :=
+    match t with
+    | tyc_prp => False
+    | tyc_arr _ _ => False
+    | _ => True
+    end.
+
+  Definition ty_rect :
+    forall P : ty -> Type,
+    P ty_prp ->
+    (forall t, P t -> forall s, P s -> P (ty_arr t s)) ->
+    (forall t, ty_other t -> P t) ->
+    forall t, P t :=
+    fun P p a (o : forall t, ty_other t -> P t) => tyc_rect P p a (o tyc_obj I).
+
+  Theorem ty_rect_prp P p a d : ty_rect P p a d ty_prp = p.
+  Proof. reflexivity. Qed.
+
+  Theorem ty_rect_arr P p a d A B :
+    ty_rect P p a d (ty_arr A B) =
+    a _ (ty_rect P p a d A) _ (ty_rect P p a d B).
+  Proof. reflexivity. Qed.
+
+  Theorem ty_rect_other P p a d t :
+    forall O : ty_other t, ty_rect P p a d t = d t O.
+  Proof.
+    intros. destruct t; simpl; destruct O. reflexivity.
+  Qed.
+End TyChurch.
+
+
+Module TyChurchTheories.
+  Module TyTheories := TyTheories TyChurch RlistList.
+  Import TyTheories.
+
+  Notation "'i'" := tyc_obj (in custom stlc_ty at level 0) : stlc_scope.
+
+  (** Examples *)
+  Check -[ o ]-.
+  Check -[ o -> i ]-.
+  Check -[ o -> (i -> o) ]-.
+  Check -[ (o -> i) -> o ]-.
+End TyChurchTheories.
